memory_safety/symbolic.v
@@ -29,34 +29,33 @@ Context {ops : machine_ops t}.
 Definition block := word t.
 
 Inductive type :=
-| TypeInt
+| TypeData
 | TypePointer : block -> type.
 
-(* CH: calling this tag would be better *)
-Inductive label :=
-| LabelValue : type -> label
-| LabelMemory : block -> type -> label
-| LabelFree.
+Inductive tag :=
+| TagValue : type -> tag
+| TagMemory : block -> type -> tag
+| TagFree.
 
-Local Notation INT := TypeInt.
+Local Notation DATA := TypeData.
 Local Notation PTR := TypePointer.
-Local Notation "V( ty )" := (LabelValue ty) (at level 4).
-Notation "M( n , ty )" := (LabelMemory n ty) (at level 4).
-Local Notation FREE := LabelFree.
-Local Notation atom := (atom (word t) label).
+Local Notation "V( ty )" := (TagValue ty) (at level 4).
+Notation "M( n , ty )" := (TagMemory n ty) (at level 4).
+Local Notation FREE := TagFree.
+Local Notation atom := (atom (word t) tag).
 
 Import PartMaps.
 
 Class abstract_params := {
   memory : Type;
-  mem_class :> partial_map memory (word t) atom;
+  mem_map :> partial_map memory (word t) atom;
   registers : Type;
-  reg_class :> partial_map registers (reg t) atom
+  reg_map :> partial_map registers (reg t) atom
 }.
 
 Class params_spec (ap : abstract_params) := {
-  mem_axioms :> PartMaps.axioms (@mem_class ap);
-  reg_axioms :> PartMaps.axioms (@reg_class ap)
+  mem_map_spec :> PartMaps.axioms (@mem_map ap);
+  reg_map_spec :> PartMaps.axioms (@reg_map ap)
 }.
 
 Context `{ap : abstract_params}
@@ -144,14 +143,14 @@ Definition mvec_match {A B} op : forall (fs : mvec_operands A (nfields op))
   end.
 
 
-Definition rules (mvec : MVec label) : option (RVec label) :=
+Definition rules (mvec : MVec tag) : option (RVec tag) :=
   match mvec with
   | mkMVec op V(PTR b) M(b',INT) ts =>
     if b == b' then
       let ret tpc tr := Some (mkRVec tpc tr) in
       let retv tr := ret V(PTR b) tr in
       mvec_match ts
-                 match op return mvec_dest _ (option (RVec label)) op with
+                 match op return mvec_dest _ (option (RVec tag)) op with
                  | NOP => retv V(INT)
                  | CONST => fun _ => retv V(INT)
                  | MOV => fun t1 t2 =>
@@ -163,40 +162,40 @@ Definition rules (mvec : MVec label) : option (RVec label) :=
                    match bo with
                    | ADD =>
                      match t1, t2 with
-                     | V(INT), V(INT) => Some (mkRVec V(PTR b) V(INT))
-                     | V(PTR b1), V(INT) => Some (mkRVec V(PTR b) V(PTR b1))
-                     | V(INT), V(PTR b2) => Some (mkRVec V(PTR b) V(PTR b2))
+                     | V(DATA), V(DATA) => Some (mkRVec V(PTR b) V(DATA))
+                     | V(PTR b1), V(DATA) => Some (mkRVec V(PTR b) V(PTR b1))
+                     | V(DATA), V(PTR b2) => Some (mkRVec V(PTR b) V(PTR b2))
                      | _, _ => None
                      end
                    | SUB =>
                      match t1, t2 with
-                     | V(INT), V(INT) => Some (mkRVec V(PTR b) V(INT))
-                     | V(PTR b1), V(INT) => Some (mkRVec V(PTR b) V(PTR b1))
+                     | V(DATA), V(DATA) => Some (mkRVec V(PTR b) V(DATA))
+                     | V(PTR b1), V(DATA) => Some (mkRVec V(PTR b) V(PTR b1))
                      | V(PTR b1), V(PTR b2) =>
-                       if b1 == b2 then Some (mkRVec V(PTR b) V(INT))
+                       if b1 == b2 then Some (mkRVec V(PTR b) V(DATA))
                        else None
                      | _, _ => None
                      end
                    | EQ =>
                      match t1, t2 with
-                     | V(INT), V(INT) => Some (mkRVec V(PTR b) V(INT))
+                     | V(DATA), V(DATA) => Some (mkRVec V(PTR b) V(DATA))
                      | V(PTR b1), V(PTR b2) =>
-                       if b1 == b2 then Some (mkRVec V(PTR b) V(INT))
+                       if b1 == b2 then Some (mkRVec V(PTR b) V(DATA))
                        else None
                      | _, _ => None
                      end
                    | LEQ =>
                      match t1, t2 with
-                     | V(INT), V(INT) => Some (mkRVec V(PTR b) V(INT))
+                     | V(DATA), V(DATA) => Some (mkRVec V(PTR b) V(DATA))
                      | V(PTR b1), V(PTR b2) =>
-                       if b1 == b2 then Some (mkRVec V(PTR b) V(INT))
+                       if b1 == b2 then Some (mkRVec V(PTR b) V(DATA))
                        else None (* comparing pointers to different regions disallowed
                                     as it would expose too much about allocation *)
                      | _, _ => None
                      end
                    | _ =>
                      match t1, t2 with
-                     | V(INT), V(INT) => Some (mkRVec V(PTR b) V(INT))
+                     | V(DATA), V(DATA) => Some (mkRVec V(PTR b) V(DATA))
                      | _, _ => None
                      end
                    end
@@ -217,12 +216,12 @@ Definition rules (mvec : MVec label) : option (RVec label) :=
                  | JUMP => fun t =>
                    match t with
                    | V(PTR b') =>
-                     ret V(PTR b') V(INT)
+                     ret V(PTR b') V(DATA)
                    | _ => None
                    end
                  | BNZ => fun t =>
                    match t with
-                   | V(INT) => retv V(INT)
+                   | V(DATA) => retv V(DATA)
                    | _ => None
                    end
                  | JAL => fun t _ =>
@@ -236,7 +235,7 @@ Definition rules (mvec : MVec label) : option (RVec label) :=
                  end
     else None
 (* CH: Would like to add this but I can't because of dependent types
-  | mkMVec SERVICE V(INT) _ ts => Some (mkRVec V(INT) V(INT))*)
+  | mkMVec SERVICE V(DATA) _ ts => Some (mkRVec V(DATA) V(DATA))*)
   | _ => None
   end.
 End WithVectorNotations.
@@ -254,7 +253,7 @@ Definition initial_state := (initial_mem, initial_registers, initial_pc@V(PTR in
 
 Definition type_eq t1 t2 :=
   match t1, t2 with
-    | TypeInt, TypeInt => true
+    | TypeData, TypeData => true
     | TypePointer b1, TypePointer b2 => b1 == b2
     | _, _ => false
   end.
@@ -265,40 +264,39 @@ Admitted.
 Definition type_eqMixin := EqMixin type_eqP.
 Canonical type_eqType := Eval hnf in EqType type type_eqMixin.
 
-Definition label_eq l1 l2 :=
+Definition tag_eq l1 l2 :=
   match l1, l2 with
-    | LabelValue t1, LabelValue t2 => t1 == t2
-    | LabelMemory b1 t1, LabelMemory b2 t2 => (b1 == b2) && (t1 == t2)
-    | LabelFree, LabelFree => true
+    | TagValue t1, TagValue t2 => t1 == t2
+    | TagMemory b1 t1, TagMemory b2 t2 => (b1 == b2) && (t1 == t2)
+    | TagFree, TagFree => true
     | _, _ => false
   end.
 
-Lemma label_eqP : Equality.axiom label_eq.
+Lemma tag_eqP : Equality.axiom tag_eq.
 Admitted.
 
-Definition label_eqMixin := EqMixin label_eqP.
-Canonical label_eqType := Eval hnf in EqType label label_eqMixin.
+Definition tag_eqMixin := EqMixin tag_eqP.
+Canonical tag_eqType := Eval hnf in EqType tag tag_eqMixin.
 
 Global Instance sym_memory_safety : symbolic_params := {
-  tag := label_eqType;
+  tag := tag_eqType;
 
   handler := rules;
 
   internal_state := (word * list block_info)%type;
 
   memory := memory;
-  sm := mem_class;
+  sm := mem_map;
 
   registers := registers;
-  sr := reg_class
+  sr := reg_map
 }.
 
 Definition malloc_fun st : option (state t) :=
-  let: pcv@pcl := pc st in
   let: (color,info) := internal st in
   do! sz <- get (regs st) syscall_arg1;
   match sz with
-    | sz@V(INT) =>
+    | sz@V(DATA) =>
       match compare 0 sz with
         | Lt =>
           if ohead [seq x <- info | ((sz <=? block_size x) && ~~ is_some (block_color x))%ordered] is Some x then
@@ -315,12 +313,13 @@ Definition malloc_fun st : option (state t) :=
           in
           let P := fun n => memory in
           let upd_fun := fun n acc =>
-            if @upd memory _ _ (@mem_class _) acc (block_base x + (Z_to_word (Z.of_nat n))) (0@M(color,INT)) is Some mem then mem else acc
+            if @upd memory _ _ (@mem_map _) acc (block_base x + (Z_to_word (Z.of_nat n))) (0@M(color,DATA)) is Some mem then mem else acc
           in
           let mem' := nat_rect P (mem st) upd_fun (Z.to_nat (word_to_Z sz)) in
-          let regs' := if @upd registers _ _ (@reg_class _) (regs st) syscall_ret ((block_base x)@V(PTR color)) is Some regs' then regs' else regs st in
+          let regs' := if @upd registers _ _ (@reg_map _) (regs st) syscall_ret ((block_base x)@V(PTR color)) is Some regs' then regs' else regs st in
           let color' := color + 1 in
-          Some (State mem' regs' (pcv.+1@pcl) (color',info'))
+          do! raddr <- get (regs st) ra;
+          Some (State mem' regs' raddr (color',info'))
           else None
         | _ => None
       end
@@ -332,7 +331,6 @@ Definition def_info : block_info :=
 
 (* TODO: avoid memory fragmentation *)
 Definition free_fun (st : state t) : option (state t) :=
-  let: pcv@pcl := pc st in
   let: (next_color,info) := internal st in
   do! ptr <- get (regs st) syscall_arg1;
     (* Removing the return clause makes Coq loop... *)
@@ -348,7 +346,8 @@ Definition free_fun (st : state t) : option (state t) :=
       let mem' := nat_rect P (mem st) upd_fun (Z.to_nat (word_to_Z (block_size x))) in
       let info' := set_nth def_info info i (mkBlockInfo (block_base x) (block_size x) None)
       in 
-      Some (State mem' (regs st) pcv.+1@pcl (next_color,info'))
+      do! raddr <- get (regs st) ra;
+      Some (State mem' (regs st) raddr (next_color,info'))
     else None
   | _ => None
   end.
@@ -356,25 +355,24 @@ Definition free_fun (st : state t) : option (state t) :=
 (* This factors out the common part of sizeof, basep, and offp *)
 Definition ptr_fun (st : state t)
     (f : block_info -> word -> atom) : option (state t) :=
-  let: pcv@pcl := pc st in
   let: (next_color,inf) := internal st in
   do! ptr <- get (regs st) syscall_arg1;
   match ptr return option (state t) with
   | ptr@V(PTR color) =>
     do! x <- ohead [seq x <- inf | block_color x == Some color];
     do! regs' <- upd (regs st) syscall_ret (f x color);
-    Some (State (mem st) regs' pcv.+1@pcl (next_color,inf))
+    do! raddr <- get (regs st) ra;
+    Some (State (mem st) regs' raddr (next_color,inf))
   | _ => None
   end.
 
 Definition sizeof_fun (st : state t) : option (state t) :=
-  ptr_fun st (fun x _ => (block_size x)@V(INT)).
+  ptr_fun st (fun x _ => (block_size x)@V(DATA)).
 
 Definition basep_fun (st : state t) : option (state t) :=
   ptr_fun st (fun x color => (block_base x)@V(PTR color)).
 
 Definition eqp_fun (st : state t) : option (state t) :=
-  let: pcv@pcl := pc st in
   let: (next_color,inf) := internal st in
   do! ptr1 <- get (regs st) syscall_arg1;
   do! ptr2 <- get (regs st) syscall_arg2;
@@ -382,17 +380,18 @@ Definition eqp_fun (st : state t) : option (state t) :=
   | ptr1@V(PTR color1), ptr2@V(PTR color2) =>
     let b := if (color1 == color2) && (ptr1 == ptr2) then Z_to_word 1%Z
              else Z_to_word 0%Z in
-    do! regs' <- upd (regs st) syscall_ret b@V(INT);
-    Some (State (mem st) regs' pcv.+1@pcl (next_color,inf))
+    do! regs' <- upd (regs st) syscall_ret b@V(DATA);
+    do! raddr <- get (regs st) ra;
+    Some (State (mem st) regs' raddr (next_color,inf))
   | _, _ => None
   end.
 
 Definition memsafe_syscalls : list (syscall t) :=
-  [Syscall malloc_addr V(INT) malloc_fun;
-   Syscall free_addr V(INT) free_fun;
-   Syscall size_addr V(INT) sizeof_fun;
-   Syscall base_addr V(INT) basep_fun;
-   Syscall eq_addr V(INT) malloc_fun].
+  [Syscall malloc_addr V(DATA) malloc_fun;
+   Syscall free_addr V(DATA) free_fun;
+   Syscall size_addr V(DATA) sizeof_fun;
+   Syscall base_addr V(DATA) basep_fun;
+   Syscall eq_addr V(DATA) malloc_fun].
 
 Definition step := step memsafe_syscalls.
 
@@ -403,10 +402,10 @@ Arguments registers t {_}.
 
 Module Notations.
 
-Notation INT := (TypeInt _).
+Notation DATA := (TypeData _).
 Notation PTR := TypePointer.
-Notation "V( ty )" := (LabelValue ty) (at level 4).
-Notation "M( n , ty )" := (LabelMemory n ty) (at level 4).
+Notation "V( ty )" := (TagValue ty) (at level 4).
+Notation "M( n , ty )" := (TagMemory n ty) (at level 4).
 
 End Notations.
 
